src/Lean/Expr.lean
@@ -5,6 +5,7 @@ Authors: Leonardo de Moura
 -/
 prelude
 import Init.Data.Hashable
+import Init.Data.Int
 import Lean.Data.KVMap
 import Lean.Data.SMap
 import Lean.Level
@@ -2140,16 +2141,13 @@ def mkInstLE : Expr := mkConst ``instLENat
 end Nat
 
 private def natAddFn : Expr :=
-  let nat := mkConst ``Nat
-  mkApp4 (mkConst ``HAdd.hAdd [0, 0, 0]) nat nat nat Nat.mkInstHAdd
+  mkApp4 (mkConst ``HAdd.hAdd [0, 0, 0]) Nat.mkType Nat.mkType Nat.mkType Nat.mkInstHAdd
 
 private def natSubFn : Expr :=
-  let nat := mkConst ``Nat
-  mkApp4 (mkConst ``HSub.hSub [0, 0, 0]) nat nat nat Nat.mkInstHSub
+  mkApp4 (mkConst ``HSub.hSub [0, 0, 0]) Nat.mkType Nat.mkType Nat.mkType Nat.mkInstHSub
 
 private def natMulFn : Expr :=
-  let nat := mkConst ``Nat
-  mkApp4 (mkConst ``HMul.hMul [0, 0, 0]) nat nat nat Nat.mkInstHMul
+  mkApp4 (mkConst ``HMul.hMul [0, 0, 0]) Nat.mkType Nat.mkType Nat.mkType Nat.mkInstHMul
 
 /-- Given `a : Nat`, returns `Nat.succ a` -/
 def mkNatSucc (a : Expr) : Expr :=
@@ -2168,17 +2166,97 @@ def mkNatMul (a b : Expr) : Expr :=
   mkApp2 natMulFn a b
 
 private def natLEPred : Expr :=
-  mkApp2 (mkConst ``LE.le [0]) (mkConst ``Nat) Nat.mkInstLE
+  mkApp2 (mkConst ``LE.le [0]) Nat.mkType Nat.mkInstLE
 
 /-- Given `a b : Nat`, return `a ≤ b` -/
 def mkNatLE (a b : Expr) : Expr :=
   mkApp2 natLEPred a b
 
 private def natEqPred : Expr :=
-  mkApp (mkConst ``Eq [1]) (mkConst ``Nat)
+  mkApp (mkConst ``Eq [1]) Nat.mkType
 
 /-- Given `a b : Nat`, return `a = b` -/
 def mkNatEq (a b : Expr) : Expr :=
   mkApp2 natEqPred a b
+
+/-! Constants for Int typeclasses. -/
+namespace Int
+
+protected def mkType : Expr := mkConst ``Int
+
+def mkInstNeg : Expr := mkConst ``Int.instNegInt
+
+def mkInstAdd : Expr := mkConst ``Int.instAdd
+def mkInstHAdd : Expr := mkApp2 (mkConst ``instHAdd [levelZero]) Int.mkType mkInstAdd
+
+def mkInstSub : Expr := mkConst ``Int.instSub
+def mkInstHSub : Expr := mkApp2 (mkConst ``instHSub [levelZero]) Int.mkType mkInstSub
+
+def mkInstMul : Expr := mkConst ``Int.instMul
+def mkInstHMul : Expr := mkApp2 (mkConst ``instHMul [levelZero]) Int.mkType mkInstMul
+
+def mkInstDiv : Expr := mkConst ``Int.instDiv
+def mkInstHDiv : Expr := mkApp2 (mkConst ``instHDiv [levelZero]) Int.mkType mkInstDiv
+
+def mkInstMod : Expr := mkConst ``Int.instMod
+def mkInstHMod : Expr := mkApp2 (mkConst ``instHMod [levelZero]) Int.mkType mkInstMod
+
+def mkInstPow : Expr := mkConst ``Int.instNatPow
+def mkInstPowNat  : Expr := mkApp2 (mkConst ``instPowNat [levelZero]) Int.mkType mkInstPow
+def mkInstHPow : Expr := mkApp3 (mkConst ``instHPow [levelZero, levelZero]) Int.mkType Nat.mkType mkInstPowNat
+
+def mkInstLT : Expr := mkConst ``Int.instLTInt
+def mkInstLE : Expr := mkConst ``Int.instLEInt
+
+end Int
+
+private def intNegFn : Expr :=
+  mkApp2 (mkConst ``Neg.neg [0]) Int.mkType Int.mkInstNeg
+
+private def intAddFn : Expr :=
+  mkApp4 (mkConst ``HAdd.hAdd [0, 0, 0]) Int.mkType Int.mkType Int.mkType Int.mkInstHAdd
+
+private def intSubFn : Expr :=
+  mkApp4 (mkConst ``HSub.hSub [0, 0, 0]) Int.mkType Int.mkType Int.mkType Int.mkInstHSub
+
+private def intMulFn : Expr :=
+  mkApp4 (mkConst ``HMul.hMul [0, 0, 0]) Int.mkType Int.mkType Int.mkType Int.mkInstHMul
+
+/-- Given `a : Int`, returns `- a` -/
+def mkIntNeg (a : Expr) : Expr :=
+  mkApp intNegFn a
+
+/-- Given `a b : Int`, returns `a + b` -/
+def mkIntAdd (a b : Expr) : Expr :=
+  mkApp2 intAddFn a b
+
+/-- Given `a b : Int`, returns `a - b` -/
+def mkIntSub (a b : Expr) : Expr :=
+  mkApp2 intSubFn a b
+
+/-- Given `a b : Int`, returns `a * b` -/
+def mkIntMul (a b : Expr) : Expr :=
+  mkApp2 intMulFn a b
+
+private def intLEPred : Expr :=
+  mkApp2 (mkConst ``LE.le [0]) Int.mkType Int.mkInstLE
+
+/-- Given `a b : Int`, return `a ≤ b` -/
+def mkIntLE (a b : Expr) : Expr :=
+  mkApp2 intLEPred a b
+
+private def intEqPred : Expr :=
+  mkApp (mkConst ``Eq [1]) Int.mkType
+
+/-- Given `a b : Int`, return `a = b` -/
+def mkIntEq (a b : Expr) : Expr :=
+  mkApp2 intEqPred a b
+
+def mkIntLit (n : Nat) : Expr :=
+  let r := mkRawNatLit n
+  mkApp3 (mkConst ``OfNat.ofNat [levelZero]) Int.mkType r (mkApp (mkConst ``instOfNat) r)
+
+def reflBoolTrue : Expr :=
+  mkApp2 (mkConst ``Eq.refl [levelOne]) (mkConst ``Bool) (mkConst ``Bool.true)
 
 end Lean
